src/guarding/point_props.v
@@ -17,6 +17,8 @@ From iris.base_logic.lib Require Export invariants.
 From iris.base_logic.lib Require Export fancy_updates.
 From iris.base_logic.lib Require Export fancy_updates_from_vs.
 
+From iris.bi Require Import derived_laws_later.
+
 From iris.proofmode Require Import coq_tactics reduction.
 From iris.proofmode Require Export tactics.
 From iris.program_logic Require Import atomic.
@@ -174,6 +176,190 @@ Proof.
   } 
 Qed.
 
+Lemma uPred_holds_later_m m (P : iProp Σ) n x
+  : n < m -> (uPred_holds (▷^m P) n x).
+Proof.
+  generalize n.
+  induction m.
+  { intros. lia. }
+  { intro n0. intro n0_lt_sm. assert ((▷^(S m) P)%I = (▷ ▷^m P)%I) by trivial. rewrite H.
+  unfold "▷". uPred.unseal.
+  unfold uPred_holds, upred.uPred_later_def.
+  destruct  n0; trivial.
+  apply IHm. lia.
+  }
+Qed.
+  
+Lemma uPred_holds_later_m2 m (P : iProp Σ) n x
+  : n >= m -> (uPred_holds (▷^m P) n x <-> uPred_holds P (n - m) x).
+Proof.
+  generalize n.
+  induction m.
+  { intros. replace (n0 - 0) with n0 by lia. trivial. }
+  { intro n0. intro n0_lt_sm. assert ((▷^(S m) P)%I = (▷ ▷^m P)%I) by trivial. rewrite H.
+  split.
+  { unfold "▷". uPred.unseal.
+    intro uh.
+    unfold uPred_holds, upred.uPred_later_def in uh.
+    destruct  n0.
+      {  lia. }
+      {  replace (S n0 - S m) with (n0 - m) by lia.
+        apply IHm. { lia. } trivial.
+      }
+    }
+  { 
+    unfold "▷". uPred.unseal.
+    intro uh.
+    unfold uPred_holds, upred.uPred_later_def.
+    destruct  n0.
+      {  lia. }
+      {  replace (S n0 - S m) with (n0 - m) by lia.
+        apply IHm. { lia. } trivial. } 
+  }
+  }
+Qed.
+  
+Lemma uPred_holds_later_m3 m (P : iProp Σ) n x
+  : uPred_holds (▷^m P) n x <-> (n < m \/ uPred_holds P (n - m) x).
+Proof.
+  have h : Decision (n < m) by solve_decision. destruct h.
+  { intuition. { apply uPred_holds_later_m. trivial. }
+      { apply uPred_holds_later_m. trivial. }
+  }
+  { intuition. { right. apply uPred_holds_later_m2. { lia. } trivial. }
+    { apply uPred_holds_later_m2. { lia. } trivial. }
+  }
+Qed.
+  
+Lemma uPred_ownM_separates_out_except0_later x (P : iProp Σ) (m: nat)
+  : (P -∗ ▷^m ◇ uPred_ownM x) ∗ P ⊢ (
+          ▷^m ((◇ uPred_ownM x) ∗ (uPred_ownM x -∗ P))).
+Proof.
+  unfold "◇". uPred.unseal.
+  split.
+  intros n x0 val t.
+  
+  unfold uPred_holds, upred.uPred_sep_def in t.
+  destruct t as [x1 [x2 [sum [t1 t2]]]].
+  
+  unfold uPred_holds, upred.uPred_wand_def in t1.
+  
+  assert (✓{n} (x1 ⋅ x2)) as val_12. { setoid_rewrite <- sum. trivial. }
+  assert (n ≤ n) as nle by trivial.
+  have t11 := t1 n x2 nle val_12 t2.
+  
+  rewrite uPred_holds_later_m3 in t11.
+  
+  unfold uPred_holds in t11. unfold upred.uPred_or_def in t11.
+  
+  have h : Decision (n < m) by solve_decision. destruct h.
+  {
+    rewrite uPred_holds_later_m3. left. trivial. 
+  }
+  
+    (*unfold uPred_holds, upred.uPred_sep_def. exists ε, x0.
+    split.
+    { rewrite ucmra_unit_left_id. trivial. }
+    split.
+    { rewrite uPred_holds_later_m3. left. trivial. }
+    unfold uPred_holds, upred.uPred_wand_def.
+    intros n' x' n'_le_n valn' uh.
+    
+    apply upred.uPred_mono with (n1 := n) (x1 := x2); trivial.
+    unfold includedN. exists (x1 ⋅ x').
+    apply dist_le with (n := n); trivial.
+    setoid_rewrite sum.
+    assert (x2 ⋅ (x1 ⋅ x') ≡ (x2 ⋅ x1 ⋅ x')) as J. { apply cmra_assoc. }
+    setoid_rewrite J.
+    
+    assert (x1 ⋅ x2 ≡ x2 ⋅ x1) as K. { apply cmra_comm. }
+    setoid_rewrite K.
+    trivial.
+  }*)
+  
+  destruct t11 as [n_lt_m|[tlatfalse|t11]].
+  { lia. }
+  {
+    unfold uPred_holds in tlatfalse. unfold upred.uPred_later_def in tlatfalse.
+    unfold uPred_holds in tlatfalse. unfold upred.uPred_pure_def in tlatfalse.
+    
+    have h : Decision (n = m) by solve_decision. destruct h.
+    2: { assert (n - m > 0) as X by lia. destruct (n-m). { lia. } contradiction. }
+    subst n.
+    
+    rewrite uPred_holds_later_m3. right.
+    
+    unfold uPred_holds, upred.uPred_sep_def. exists ε, x0.
+    split.
+    { rewrite ucmra_unit_left_id. trivial. }
+    split.
+    { unfold uPred_holds, upred.uPred_or_def. left. unfold uPred_holds, upred.uPred_later_def. trivial. }
+    unfold uPred_holds, upred.uPred_wand_def.
+    intros n' x' le_m valxx uh.
+    apply uPred_mono with (n1 := m) (x1 := x0 ⋅ x'); trivial.
+    {
+    setoid_rewrite sum.
+    eapply uPred_mono. { apply t2. }
+    { unfold includedN. exists (x1 ⋅ x').
+      assert (x2 ⋅ (x1 ⋅ x') ≡ (x2 ⋅ x1 ⋅ x')) as J. { apply cmra_assoc. }
+      setoid_rewrite J.
+      assert (x1 ⋅ x2 ≡ x2 ⋅ x1) as K. { apply cmra_comm. }
+      setoid_rewrite K.
+      trivial.
+    }
+    lia.
+    }
+    lia.
+  } 
+  
+  unfold uPred_holds in t11. unfold upred.uPred_ownM_def in t11.
+  unfold includedN in t11. destruct t11 as [z h].
+  
+  rewrite uPred_holds_later_m3. right.
+  
+  unfold uPred_holds. unfold upred.uPred_sep_def.
+  destruct (cmra_extend (n-m) (x1 ⋅ x2) x z) as (xe&ze&Hx'&Hy1&Hy2); trivial.
+  { apply cmra_validN_le with (n := n); trivial. lia. }
+  
+  exists xe. exists ze.
+  
+  split.
+  { setoid_rewrite <- Hx'.
+      apply dist_le with (n := n); trivial. lia. }
+  split.
+  { unfold uPred_holds, upred.uPred_or_def. right.
+      unfold uPred_holds, upred.uPred_ownM_def.
+        setoid_rewrite Hy1. trivial. }
+  { unfold uPred_holds, upred.uPred_wand_def.
+    intros n' x' incl val2 uh.
+      unfold uPred_holds in uh.
+      unfold upred.uPred_ownM_def in uh.
+      unfold includedN in uh. destruct uh as [w j].
+      setoid_rewrite j.
+       
+      assert (uPred_holds P n x0) as ux0. {
+        eapply uPred_mono. { apply t2. }
+        { setoid_rewrite sum. unfold includedN. exists x1.
+            rewrite cmra_comm. trivial. }
+        trivial.
+      }
+       
+      apply uPred_mono with (n1 := n) (x1 := x0); trivial.
+      { 
+      assert (ze ⋅ (x ⋅ w) ≡ (ze ⋅ x) ⋅ w) as associ. { apply cmra_assoc. }
+      setoid_rewrite associ.
+      assert ((ze ⋅ x) ≡ (x ⋅ ze)) as commu. { apply cmra_comm. }
+      setoid_rewrite commu.
+      unfold includedN. exists w.
+      apply dist_le with (n := n - m); trivial.
+      setoid_rewrite <- Hy1.
+      setoid_rewrite <- Hx'.
+      apply dist_le with (n := n); trivial.
+      { setoid_rewrite sum. trivial. }
+      lia.
+      } lia.
+  } 
+Qed.
 
 
 (* For the "Point Proposition" formulation from the paper *)
@@ -235,6 +421,16 @@ Lemma own_separates_out_except0_point (P : iProp Σ) (Q: iProp Σ)
 Proof.
   unfold point_prop in point. destruct point as [x point]. setoid_rewrite point.
   apply uPred_ownM_separates_out_except0.
+Qed.
+
+Lemma own_separates_out_except0_point_later (P : iProp Σ) (Q: iProp Σ) (n: nat)
+    (point: point_prop Q)
+  : (P -∗ ▷^n ◇ Q) ∗ P ⊢ (
+          ▷^n (◇ Q ∗ (Q -∗ P))
+      ).
+Proof.
+  unfold point_prop in point. destruct point as [x point]. setoid_rewrite point.
+  apply uPred_ownM_separates_out_except0_later.
 Qed.
 
 End SeparableAnd.
